NLustre.v
@@ -1,17 +1,19 @@
-Require Import Operators.
-Require Import Clocks.
+Require Export Operators.
+Require Export Clocks.
 Require Export NLustre.Stream.
-Require Import NLustre.NLExprSyntax.
+Require Export NLustre.NLExprSyntax.
 Require Export NLustre.NLSyntax.
+Require Export NLustre.IsFreeExpr.
 Require Export NLustre.IsFree.
 Require Export NLustre.IsVariable.
 Require Export NLustre.IsDefined.
 Require Export NLustre.Memories.
-Require Import NLustre.NLExprSemantics.
+Require Export NLustre.NLExprSemantics.
 Require Export NLustre.NLSemantics.
 Require Export NLustre.MemSemantics.
 Require Export NLustre.Ordered.
 Require Export NLustre.NoDup.
+Require Export NLustre.NLClockingExpr.
 Require Export NLustre.NLClocking.
 Require Export NLustre.NLClockingSemantics.
 Require Export NLustre.NLTyping.
@@ -25,21 +27,23 @@ Module Type NLUSTRE
        (Clks   : CLOCKS         Ids)
        (ExprSyn: NLEXPRSYNTAX        Op)
        (Str    : STREAM              Op OpAux)
-       (ExprSem: NLEXPRSEMANTICS Ids Op OpAux Clks ExprSyn Str).
+       (ExprSem: NLEXPRSEMANTICS Ids Op OpAux Clks ExprSyn Str)
+       (IsFExpr: ISFREEEXPR      Ids Op       Clks ExprSyn)
+       (CloExpr: NLCLOCKINGEXPR  Ids Op       Clks ExprSyn).
 
   Declare Module Export Syn    : NLSYNTAX        Ids Op       Clks ExprSyn.
   Declare Module Export Ord    : ORDERED         Ids Op       Clks ExprSyn Syn.
-  Declare Module Export IsF    : ISFREE          Ids Op       Clks ExprSyn Syn.
+  Declare Module Export IsF    : ISFREE          Ids Op       Clks ExprSyn Syn IsFExpr.
   Declare Module Export Sem    : NLSEMANTICS     Ids Op OpAux Clks ExprSyn Syn Str Ord ExprSem.
   Declare Module Export Typ    : NLTYPING        Ids Op       Clks ExprSyn Syn.
   Declare Module Export Mem    : MEMORIES        Ids Op       Clks ExprSyn Syn.
   Declare Module Export IsD    : ISDEFINED       Ids Op       Clks ExprSyn Syn                     Mem.
   Declare Module Export IsV    : ISVARIABLE      Ids Op       Clks ExprSyn Syn                     Mem IsD.
   Declare Module Export NoD    : NODUP           Ids Op       Clks ExprSyn Syn                     Mem IsD IsV.
-  Declare Module Export Clo    : NLCLOCKING      Ids Op       Clks ExprSyn Syn     Ord             Mem IsD     IsF.
+  Declare Module Export Clo    : NLCLOCKING      Ids Op       Clks ExprSyn Syn     Ord             Mem IsD IsFExpr IsF CloExpr.
   Declare Module Export CloSem : NLCLOCKINGSEMANTICS Ids Op OpAux Clks ExprSyn Syn
-                                                     Str Ord ExprSem Sem Mem IsD  IsF Clo.
-  Declare Module Export MemSem : MEMSEMANTICS    Ids Op OpAux Clks ExprSyn Syn Str Ord ExprSem Sem Mem IsD IsV IsF NoD Clo CloSem.
+                                                     Str Ord ExprSem Sem Mem IsD IsFExpr IsF CloExpr Clo.
+  Declare Module Export MemSem : MEMSEMANTICS    Ids Op OpAux Clks ExprSyn Syn Str Ord ExprSem Sem Mem IsD IsV IsFExpr IsF NoD CloExpr Clo CloSem.
 
 End NLUSTRE.
 
@@ -51,19 +55,21 @@ Module NLustreFun
        (ExprSyn: NLEXPRSYNTAX  Op)
        (Str    : STREAM              Op OpAux)
        (ExprSem: NLEXPRSEMANTICS Ids Op OpAux Clks ExprSyn Str)
-       <: NLUSTRE Ids Op OpAux Clks ExprSyn Str ExprSem.
+       (IsFExpr: ISFREEEXPR      Ids Op       Clks ExprSyn)
+       (CloExpr: NLCLOCKINGEXPR  Ids Op       Clks ExprSyn)
+<: NLUSTRE Ids Op OpAux Clks ExprSyn Str ExprSem IsFExpr CloExpr.
   Module Export Syn     := NLSyntaxFun        Ids Op       Clks ExprSyn.
   Module Export Ord     := OrderedFun         Ids Op       Clks ExprSyn Syn.
-  Module Export IsF     := IsFreeFun          Ids Op       Clks ExprSyn Syn.
+  Module Export IsF     := IsFreeFun          Ids Op       Clks ExprSyn Syn IsFExpr.
   Module Export Sem     := NLSemanticsFun     Ids Op OpAux Clks ExprSyn Syn Str Ord ExprSem.
   Module Export Typ     := NLTypingFun        Ids Op       Clks ExprSyn Syn.
   Module Export Mem     := MemoriesFun        Ids Op       Clks ExprSyn Syn.
   Module Export IsD     := IsDefinedFun       Ids Op       Clks ExprSyn Syn                     Mem.
   Module Export IsV     := IsVariableFun      Ids Op       Clks ExprSyn Syn                     Mem IsD.
   Module Export NoD     := NoDupFun           Ids Op       Clks ExprSyn Syn                     Mem IsD IsV.
-  Module Export Clo     := NLClockingFun      Ids Op       Clks ExprSyn Syn     Ord             Mem IsD     IsF.
+  Module Export Clo     := NLClockingFun      Ids Op       Clks ExprSyn Syn     Ord             Mem IsD IsFExpr IsF CloExpr.
   Module Export CloSem  := NLClockingSemanticsFun Ids Op OpAux Clks ExprSyn Syn
-                                                  Str Ord ExprSem Sem Mem IsD  IsF Clo.
-  Module Export MemSem  := MemSemanticsFun    Ids Op OpAux Clks ExprSyn Syn Str Ord ExprSem Sem Mem IsD IsV IsF NoD Clo CloSem.
+                                                     Str Ord ExprSem Sem Mem IsD IsFExpr IsF CloExpr Clo.
+  Module Export MemSem  := MemSemanticsFun    Ids Op OpAux Clks ExprSyn Syn Str Ord ExprSem Sem Mem IsD IsV IsFExpr IsF NoD CloExpr Clo CloSem.
 
 End NLustreFun.
