SyBloc.v
@@ -1,21 +1,22 @@
-Require Import Velus.Common.
-Require Import Velus.Operators.
-Require Import Velus.Clocks.
+Require Export Velus.Common.
+Require Export Velus.Operators.
+Require Export Velus.Clocks.
 Require Export Velus.NLustre.Stream.
-Require Import Velus.NLustre.NLExprSyntax.
-Require Import Velus.SyBloc.SBSyntax.
-Require Import Velus.SyBloc.SBIsBlock.
-Require Import Velus.SyBloc.SBOrdered.
-Require Import Velus.NLustre.NLExprSemantics.
-Require Import Velus.SyBloc.SBSemantics.
-Require Import Velus.SyBloc.SBIsLast.
-Require Import Velus.SyBloc.SBIsVariable.
-Require Import Velus.SyBloc.SBIsDefined.
-Require Import Velus.NLustre.NLSyntax.
-Require Import Velus.NLustre.IsFree.
-Require Import Velus.SyBloc.SBIsFree.
-Require Import Velus.SyBloc.SBWellDefined.
-Require Import Velus.SyBloc.SBSchedule.
+Require Export Velus.NLustre.NLExprSyntax.
+Require Export Velus.SyBloc.SBSyntax.
+Require Export Velus.SyBloc.SBIsBlock.
+Require Export Velus.SyBloc.SBOrdered.
+Require Export Velus.NLustre.NLExprSemantics.
+Require Export Velus.SyBloc.SBSemantics.
+Require Export Velus.SyBloc.SBIsLast.
+Require Export Velus.SyBloc.SBIsVariable.
+Require Export Velus.SyBloc.SBIsDefined.
+Require Export Velus.NLustre.IsFreeExpr.
+Require Export Velus.SyBloc.SBIsFree.
+Require Export Velus.SyBloc.SBWellDefined.
+Require Export Velus.SyBloc.SBSchedule.
+Require Export Velus.NLustre.NLClockingExpr.
+Require Export Velus.SyBloc.SBClocking.
 
 Module Type SYBLOC
        (Ids    : IDS)
@@ -25,8 +26,8 @@ Module Type SYBLOC
        (ExprSyn: NLEXPRSYNTAX        Op)
        (Str    : STREAM              Op OpAux)
        (ExprSem: NLEXPRSEMANTICS Ids Op OpAux Clks ExprSyn Str)
-       (SynNL  : NLSYNTAX        Ids Op       Clks ExprSyn)
-       (FreeNL : ISFREE          Ids Op       Clks ExprSyn     SynNL).
+       (IsFExpr: ISFREEEXPR      Ids Op       Clks ExprSyn)
+       (CloExpr: NLCLOCKINGEXPR  Ids Op       Clks ExprSyn).
 
   Declare Module Export Syn  : SBSYNTAX      Ids Op       Clks ExprSyn.
   Declare Module Export Block: SBISBLOCK     Ids Op       Clks ExprSyn Syn.
@@ -35,8 +36,9 @@ Module Type SYBLOC
   Declare Module Export Last : SBISLAST      Ids Op       Clks ExprSyn Syn.
   Declare Module Export Var  : SBISVARIABLE  Ids Op       Clks ExprSyn Syn.
   Declare Module Export Def  : SBISDEFINED   Ids Op       Clks ExprSyn Syn Var Last.
-  Declare Module Export Free : SBISFREE      Ids Op       Clks ExprSyn Syn SynNL FreeNL.
-  Declare Module Export Wdef : SBWELLDEFINED Ids Op       Clks ExprSyn Syn Block Ord Var Last Def SynNL FreeNL Free.
+  Declare Module Export Free : SBISFREE      Ids Op       Clks ExprSyn Syn IsFExpr.
+  Declare Module Export Wdef : SBWELLDEFINED Ids Op       Clks ExprSyn Syn Block Ord Var Last Def IsFExpr Free.
+  Declare Module Export Clo  : SBCLOCKING    Ids Op       Clks ExprSyn Syn Last Var Def CloExpr.
 
   Declare Module Scheduler   : SBSCHEDULE    Ids Op OpAux Clks ExprSyn Syn Block Ord Str ExprSem Sem.
 
@@ -45,14 +47,14 @@ End SYBLOC.
 Module SyBlocFun
        (Ids    : IDS)
        (Op     : OPERATORS)
-       (OpAux  : OPERATORS_AUX Op)
-       (Clks   : CLOCKS    Ids)
-       (ExprSyn: NLEXPRSYNTAX  Op)
+       (OpAux  : OPERATORS_AUX       Op)
+       (Clks   : CLOCKS          Ids)
+       (ExprSyn: NLEXPRSYNTAX        Op)
        (Str    : STREAM              Op OpAux)
        (ExprSem: NLEXPRSEMANTICS Ids Op OpAux Clks ExprSyn Str)
-       (SynNL  : NLSYNTAX  Ids Op Clks ExprSyn)
-       (FreeNL : ISFREE    Ids Op Clks ExprSyn SynNL)
-<: SYBLOC Ids Op OpAux Clks ExprSyn Str ExprSem SynNL FreeNL.
+       (IsFExpr: ISFREEEXPR      Ids Op       Clks ExprSyn)
+       (CloExpr: NLCLOCKINGEXPR  Ids Op       Clks ExprSyn)
+<: SYBLOC Ids Op OpAux Clks ExprSyn Str ExprSem IsFExpr CloExpr.
 
   Module Export Syn   := SBSyntaxFun      Ids Op       Clks ExprSyn.
   Module Export Block := SBIsBlockFun     Ids Op       Clks ExprSyn Syn.
@@ -61,8 +63,9 @@ Module SyBlocFun
   Module Export Last  := SBIsLastFun      Ids Op       Clks ExprSyn Syn.
   Module Export Var   := SBIsVariableFun  Ids Op       Clks ExprSyn Syn.
   Module Export Def   := SBIsDefinedFun   Ids Op       Clks ExprSyn Syn Var Last.
-  Module Export Free  := SBIsFreeFun      Ids Op       Clks ExprSyn Syn SynNL FreeNL.
-  Module Export Wdef  := SBWellDefinedFun Ids Op       Clks ExprSyn Syn Block Ord Var Last Def SynNL FreeNL Free.
+  Module Export Free  := SBIsFreeFun      Ids Op       Clks ExprSyn Syn IsFExpr.
+  Module Export Wdef  := SBWellDefinedFun Ids Op       Clks ExprSyn Syn Block Ord Var Last Def IsFExpr Free.
+  Module Export Clo   := SBClockingFun    Ids Op       Clks ExprSyn Syn Last Var Def CloExpr.
 
   Module Scheduler    := SBScheduleFun    Ids Op OpAux Clks ExprSyn Syn Block Ord Str ExprSem Sem.
 End SyBlocFun.
